---
title: 微分方程数值解作业 2
tags: 
    - 微分方程
---

## Problem 1

![](https://cdn.duanyll.com/img/20240323155913.png)

To solve (2.4)

$$
\frac{\d^2y}{\d x^2}+p(x)\frac{\d y}{\d x}+q(x)y=f(x)
$$

We can always obtain the equation at non-boundary positions, 

$$
c_iy_{i+1}+a_iy_i+b_iy_{i-1}=h^2f(x_i), \mathrm{where}\begin{cases}
    a_i&=-2+h^2q(x_i)\\
    b_i&=1-\frac{h}{2}p(x_i)\\
    c_i&=1+\frac{h}{2}p(x_i)
\end{cases}
\label{eqn1}
$$

The above FDE approximation has an error of $O(h^2)$

### Question (a)

The first condition

$$
y(0)=\alpha\implies y_0=\alpha
$$

and $i=1$ in Eqn. $\ref{eqn1}$ becomes

$$
c_1 y_2+a_1y_1=h^2f_1-b_1\alpha.
$$

For the second condition

$$
y(\ell)+\gamma y'(\ell)=\beta,
$$

substitute $y'(\ell)$ with an one-sided approximation

$$
y'(x_{n+1})\approx\frac{3y_{n+1}-4y_n+y_{n-1}}{2h}
$$

we have

$$
y_{n+1}+\frac{\gamma}{2h}(3y_{n+1}-4y_n+y_{n-1})=\beta\implies y_{n+1}=\frac{2h\beta-\gamma y_{n-1}+4\gamma y_n}{2h+3\gamma} 
$$

And the final equation becomes

$$
c_n\frac{2h\beta-\gamma y_{n-1}+4\gamma y_n}{2h+3\gamma}+a_ny_n+b_ny_{n-1}=h^2f(x_n)
$$

$$
(b_n-\frac{c_n\gamma}{2h+3\gamma})y_{n-1}+(a_n+\frac{4\gamma c_n}{2h+3\gamma})y_n=h^2f_n-\frac{2c_nh\beta}{2h+3\gamma}
$$

The whole FDE system in matrix form

$$
\begin{pmatrix}
    a_1 & c_1 & & & &  \\
    b_2 & a_2 & c_2 & & &  \\
    & b_3 & a_3 & c_3 & &  \\
    & & \ddots & \ddots & \ddots &  \\
    & & & b_{n-1} & a_{n-1} & c_{n-1} \\
    & & & & b_n-\frac{c_N\gamma}{2h+3\gamma} & a_n+\frac{\gamma c_n}{2h+3\gamma}
\end{pmatrix}\mathbf{y}=\begin{pmatrix}
    h^2f_1-\alpha b_1 \\
    h^2f_2 \\
    h^2f_3 \\
    \vdots \\
    h^2f_{n-1} \\
    h^2f_n-\frac{2c_nh\beta}{2h+3\gamma}
\end{pmatrix}
$$

### Question (b)

$$
\begin{cases}
    y(0)=y(\ell)\\
    y'(0)=y'(\ell)
\end{cases}\implies
\begin{cases}
    y_0=y_{n+1}\\
    \frac{1}{2h}(-y_2+4y_1-3y_0)=\frac{1}{2h}(3y_{n+1}-4y_n+y_{n-1})
\end{cases}
$$

Therefore

$$
y_0=y_{n+1}=\frac{4y_1-y_2+4y_n-y_{n-1}}{6}
$$

FDE system in matrix form

$$
\begin{pmatrix}
    a_1+\frac{2}{3}b_1 &  c_1-\frac{b_1}{6} & & & -\frac{b_1}{6} & \frac{2}{3}b_1 \\
    & b_2 & a_2 & c_2 & &\\
    & & \ddots & \ddots & \ddots &\\
    & & & b_{n-1} & a_{n-1} & c_{n-1}\\
    \frac{2}{3}c_n & -\frac{c_n}{6} & & & b_n-\frac{c_n}{6} & a_n+\frac{2}{3}c_n
\end{pmatrix}\mathbf{y}=\begin{pmatrix}
    h^2f_1\\
    h^2f_2\\
    \vdots\\
    h^2f_{n-1}\\
    h^2f_n
\end{pmatrix}
$$
  
## Problem 2

![](https://cdn.duanyll.com/img/20240323155945.png)

### Question (a)

$$
\begin{aligned}
    y(x_{i+1})-2y(x_i)+y(x_{i-1})=&y(x_i)+hy'(x_i)+\frac{h^2}{2}y''(x_i)+\frac{h^3}{6}y'''(x_i)+\frac{h^4}{24}y''''(x_i)\\
    &+\frac{h^5}{120}y^{(5)}(x_i)+O(h^6)-2y(x_i)+y(x_i)-hy'(x_i)\\
    &+\frac{h^2}{2}y''(x_i)-\frac{h^3}{6}y'''(x_i)+\frac{h^4}{24}y''''(x_i)-\frac{h^5}{120}y^{(5)}(x_i)+O(h^6)\\
    =&h^2y''(x_i)+\frac{h^4}{12}y''''(x_i)+O(h^6)
\end{aligned}
$$

Use central difference to approximate $y''''(x_i)$ with $y''(x_i)$

$$
y''''(x_i)=\frac{1}{h^2}(y''(x_{i+1})-2y''(x_i)+y''(x_{i-1}))+O(h^2)
$$

Substitute back

$$
\begin{aligned}
    y(x_{i+1})-2y(x_i)+y(x_{i-1})&=h^2y''(x_i)+\frac{h^4}{12}\frac{1}{h^2}(y''(x_{i+1})-2y''(x_i)+y''(x_{i-1}))+O(h^6)\\
    &=\frac{h^2}{12}(y''(x_{i+1})+10y''(x_i)+y''(x_{i-1}))+O(h^6)
\end{aligned}
$$

### Question (b)

Given the differerntial equation

$$
y''=F(x,y)
$$

Simply susbtitute $y''$ with $F(x,y)$ in the above equation, and discard the higher order terms, we have

$$
y_{i+1}-2y_i+y_{i-1}=\frac{h^2}{12}(F_{i+1}+10F_i+F_{i-1})
$$

### Question (c)

When

$$
F(x,t)=f(x)-q(x)y
$$

we will be able to seperate $y_i$ from $F_i$, and the difference equation becomes

$$
y_{i+1}-2y_i+y_{i-1}=\frac{h^2}{12}(f_{i+1}+10f_i+f_{i-1})-\frac{h^2}{12}(q_{i+1}y_{i+1}+10q_iy_i+q_{i-1}y_{i-1})
$$

Collect $y_i$ terms on the left hand side

$$
(1+\frac{h^2}{12}q_{i+1})y_{i+1}-(2-\frac{5h^2}{6}q_i)y_i+(1+\frac{h^2}{12}q_{i-1})y_{i-1}=\frac{h^2}{12}(f_{i+1}+10f_i+f_{i-1})
\label{eqn2}
$$

The above equation is linear, and could be written in matrix form. Denote 

$$
\begin{cases}
    a_i=-(2-\frac{5h^2}{6}q_i)\\
    b_i=1+\frac{h^2}{12}q_{i-1}\\
    c_i=1+\frac{h^2}{12}q_{i+1}
\end{cases}
$$

Assume the boundary conditions are $y_0=\alpha$ and $y_N=\beta$, we can obtain Equation $\ref{eqn2}$ at $i=1$ and $i=N$

$$
\begin{aligned}
    c_1y_2+b_1y_1&=\frac{h^2}{12}(f_2+10f_1+f_0)-a_1\alpha\\
    a_{N}y_{N-1}+b_{N}y_{N}&=\frac{h^2}{12}(f_{N-1}+10f_{N}+f_{N+1})-c_{N}\beta
\end{aligned}
$$

Finally, the FDE system is expressed in explicit matrix form

$$
\begin{pmatrix}
    a_1 & c_1 & & & &  \\
    b_2 & a_2 & c_2 & & &  \\
    & b_3 & a_3 & c_3 & &  \\
    & & \ddots & \ddots & \ddots &  \\
    & & & b_{N-1} & a_{N-1} & c_{N-1} \\
    & & & & b_N & a_N
\end{pmatrix}\mathbf{y}=\begin{pmatrix}
    \frac{h^2}{12}(f_2+10f_1+f_0)-a_1\alpha\\
    \frac{h^2}{12}(f_3+10f_2+f_1)\\
    \frac{h^2}{12}(f_4+10f_3+f_2)\\
    \vdots \\
    \frac{h^2}{12}(f_{N}+10f_{N-1}+f_{N-2})\\
    \frac{h^2}{12}(f_{N-1}+10f_{N}+f_{N+1})-c_{N}
\end{pmatrix}
$$

### Question (d)

$$
y=u(x)e^{-\frac{1}{2}\int^xp(x)\d x}
$$

$$
\frac{\p y}{\p x}=-\frac{1}{2} e^{-\frac{1}{2} x p(x)} \left(x u(x) p'(x)+p(x) u(x)-2 u'(x)\right)
$$

$$
\begin{aligned}
    \frac{\p^2 y}{\p x^2}=&\frac{1}{4} e^{-\frac{1}{2} x p(x)} (2 p(x) \left(x u(x) p'(x)-2 u'(x)\right)-4 x p'(x) u'(x)\\
    &+u(x) \left(-2 x p''(x)+x^2 p'(x)^2-4 p'(x)\right)+p(x)^2 u(x)+4 u''(x))
\end{aligned}
$$

$$
\begin{aligned}    
\frac{\p^2 y}{\p x^2}+p(x)\frac{\p y}{\p x}=&\frac{1}{4} e^{-\frac{1}{2} x p(x)}(-4 x p'(x) u'(x)\\
&+u(x) \left(-2 x p''(x)+x^2 p'(x)^2-4 p'(x)\right)-p(x)^2 u(x)+4 u''(x))
\end{aligned}
$$

Therefore, when $p(x)$ satisfies $p'(x)=0$, Equation (2.4) will not contain $u'(x)$ term, and can be solve by the method in Question (b). That requires $p(x)$ to be a constant.

## Problem 3

![](https://cdn.duanyll.com/img/20240323160010.png)

At $y_1$, use a third-ordered forward difference to approximiate $y'$ and $(y')^2$

$$
\begin{aligned}
    y_1'&=\frac{1}{h}(-\frac{11}{6}y_1+3y_2-\frac{3}{2}y_3+\frac{1}{3}y_4)+O(h^3)\\
    (y_1')^2&=\frac{1}{h^2}(-\frac{11}{6}y_1+3y_2-\frac{3}{2}y_3+\frac{1}{3}y_4)^2+O(h^2)
\end{aligned}
$$

And use a forth-ordered forward difference to approximiate $y'''$

$$
y'''_1=\frac{1}{h^3}(\frac{5}{2}y_1+9y_2-12y_3+7y_4-\frac{3}{2}y_5)+O(h^2)
$$

Substitute back to the equation we have one equation

$$
y_1'''+y_1y_1'+\beta(1-(y_1')^2)=0\label{eqn3}
$$

with 5 variables $y_1$ to $y_5$.

At $y_2$ to $y_N$, use a forth-ordered central difference to approximiate $y'$ and $(y')^2$

$$
\begin{aligned}
    y_i'&=\frac{1}{h}(\frac{1}{12}y_{i-2}-\frac{2}{3}y_{i-1}+\frac{2}{3}y_{i+1}-\frac{1}{12}y_{i+2})+O(h^4)\\
    (y_i')^2&=\frac{1}{h^2}(\frac{1}{12}y_{i-2}-\frac{2}{3}y_{i-1}+\frac{2}{3}y_{i+1}-\frac{1}{12}y_{i+2})+O(h^3)
\end{aligned}
$$

and a forth-ordered central difference to approximiate $y'''$

$$
y'''_i=\frac{1}{h^3}(-\frac{1}{2}y_{i-2}+y_{i-1}-y_{i+1}+\frac{1}{2}y_{i+2})
$$

substitute them back we have $N-1$ equations

$$
y_i'''+y_iy_i'+\beta(1-(y_i')^2)=0,i=2,3,\cdots,N\label{eqn4}
$$

with $N+3$ variables from $y_0$ to $y_{N+2}$.

Also, the boundry conditions provide 3 equations

$$
\begin{aligned}
    y_0&=0\\
    \frac{1}{h}(-\frac{3}{2}y_0+2y_1-\frac{1}{2}y_2)&=0\\
    \frac{1}{h}(-\frac{1}{2}y_N+\frac{1}{2}y_{N+2})&=1
\end{aligned}\label{eqn5}
$$

Put Equations $\ref{eqn3},\ref{eqn4},\ref{eqn5}$ together, we could obtain a second-order non-linear FDE system with $N+3$ equations and $N+3$ variables $y_0$ to $y_{N+2}$. 

## Problem 4

![](https://cdn.duanyll.com/img/20240323160104.png)

### Question (a)

```mathematica
eqn = \[Epsilon] D[y[x], {x, 2}] - D[y[x], x] == -1 && y[0] == 1 && 
   y[1] == 3;
sol = (1 + # + (E^(#/\[Epsilon]) - 1)/(E^(1/\[Epsilon]) - 1)) &;
eqn /. {y -> sol}
```

```mathematica
True
```

### Question (b)

$$
\frac{\epsilon}{h^2}(y_{i+1}-2y_i+y_{i-1})+O(h)-\frac{1}{h}(y_i-y_{i-1})+O(h)=-1
$$

Collect $y_i$ terms

$$
(\frac{1}{h}+\frac{\epsilon}{h^2})y_{i-1}-(\frac{1}{h}+\frac{2\epsilon}{h^2})y_i+\frac{\epsilon}{h^2}y_{i+1}=-1
$$

$$
(h+\epsilon)y_{i-1}-(h+2\epsilon)y_i+\epsilon y_{i+1}=-h^2
$$

At boundries

$$
\begin{aligned}
    -(h+2\epsilon)y_1+\epsilon y_2&=-h^2-h-\epsilon\\
    (h+\epsilon)y_{N-1}-(h+2\epsilon)y_N&=-h^2-3\epsilon
\end{aligned}
$$

FDE system in matrix form

$$
\begin{pmatrix}
    -(h+2\epsilon) & \epsilon & & &  \\
    h+\epsilon & -(h+2\epsilon) & \epsilon & &  \\
     & \ddots & \ddots & \ddots &  \\
     & & h+\epsilon & -(h+2\epsilon) & \epsilon \\
     & & & h+\epsilon & -(h+2\epsilon)
\end{pmatrix}\mathbf{y}=\begin{pmatrix}
    -h^2-h-\epsilon \\
    -h^2 \\
    \vdots \\
    -h^2\\
    -h^2-3\epsilon
\end{pmatrix}
\label{eqn6}
$$

Since we have used first-ordered backward difference to approximate $y'$, the truncation error is $O(h)$.

### Question (c)

It is obvious that the matrix in Equation $\ref{eqn6}$ meets the second condition of Theorem 2.1, therefore the matrix is invertible.

If we use Equation (2.16) to build the FDE system, Theorem 2.2 guarantees the existence of a unique solution if $hp_{\infty}<2$. That is, $h<2\epsilon$.

### Question (d)

```mathematica
tridiagonalSolve[b_, a_, c_, z_] := Module[{y, v, w, n},
   n = Length[a];
   w = a[[1]];
   y = ConstantArray[0, n];
   y[[1]] = z[[1]]/w;
   v = ConstantArray[0, n];
   Do[
    v[[i]] = c[[i - 1]]/w;
    w = a[[i]] - b[[i]] v[[i]];
    y[[i]] = (z[[i]] - b[[i]] y[[i - 1]])/w;
    , {i, 2, n}];
   Do[
    y[[i]] = y[[i]] - v[[i + 1]] y[[i + 1]];
    , {i, n - 1, 1, -1}];
   Return[y];
   ];
```

```mathematica
solve1[\[Epsilon]_, n_] := Module[{c, a, b, h, x, y, z},
   h = 1/(n + 1);
   x = Range[h, 1 - h, h];
   b = ConstantArray[h + \[Epsilon], n];
   a = ConstantArray[-(h + 2 \[Epsilon]), n];
   c = ConstantArray[\[Epsilon], n];
   z = ConstantArray[-h^2, n];
   z[[1]] = -h^2 - h - \[Epsilon];
   z[[n]] = -h^2 - 3 \[Epsilon];
   y = tridiagonalSolve[b, a, c, z];
   Return[
    Interpolation[Join[{{0, 1}, {1, 3}}, Transpose[{x, y}]], 
     InterpolationOrder -> 1]];
   ];
solve2[\[Epsilon]_, n_] := Module[{c, a, b, h, x, y, z},
   h = 1/(n + 1);
   x = Range[h, 1 - h, h];
   b = ConstantArray[\[Epsilon] + h/2, n];
   a = ConstantArray[-2 \[Epsilon], n];
   c = ConstantArray[\[Epsilon] - h/2, n];
   z = ConstantArray[-h^2, n];
   z[[1]] = -h^2 - b[[1]];
   z[[n]] = -h^2 - 3 c[[n]];
   y = tridiagonalSolve[b, a, c, z];
   Return[
    Interpolation[Join[{{0, 1}, {1, 3}}, Transpose[{x, y}]], 
     InterpolationOrder -> 1]];
   ];
```

```mathematica
solveAndPlot[eps_, n_] := Module[{s1, s2},
  s1 = solve1[eps, n];
  s2 = solve2[eps, n];
  Plot[{symSol /. \[Epsilon] -> eps, s1[x], s2[x]}, {x, 0, 1}, 
   PlotLegends -> 
    Placed[{"Symbolic", "Method from (b)", "Equation (2.16)"}, Right],
    PlotLabel -> 
    StringForm["Solution for \[Epsilon]=``, N=``", eps, n]]
  ];
GraphicsColumn[{solveAndPlot[0.1, 10], solveAndPlot[0.1, 20], 
  solveAndPlot[0.1, 40]}]
```

![](https://cdn.duanyll.com/img/20240401105323.png)

### Question (e)

```mathematica
GraphicsColumn[{solveAndPlot[0.01, 10], solveAndPlot[0.01, 20], 
  solveAndPlot[0.01, 40]}]
```

![](https://cdn.duanyll.com/img/20240401105345.png)

### Question (f)

It can be observed that both methods are converging to the symbolic solution as $N$ increases. The method in (b) is less accurate than Equation (2.16) when $\epsilon$ is $0.1$. However, when $\epsilon$ gets smaller, (b) is still stable but Equation (2.16) oscillates. When $\epsilon$ is even smaller, (2.16) oscillates more severely.

![](https://cdn.duanyll.com/img/20240401113734.png)

The oscillation in (2.16) happens when $hp_{\infty}<2$ is violated. Therefore, when $\epsilon$ is small, the method in (b) better than (2.16) since it converges regardless of $\epsilon$ and $h$.