---
title: 微分方程数值解作业 5
tags:
  - 微分方程
tikzjax: true
---

## Problem 1

![](https://cdn.duanyll.com/img/20240513093730.png)

| Question | Dispersion Relation              | Phase Velocity                     | Group Velocity                                   | Dispersive | Dissipative |
| -------- | -------------------------------- | ---------------------------------- | ------------------------------------------------ | ---------- | ----------- |
| (a)      | $-gk+k^3\mu+\omega=0$            | $g+\mu k^2$                        | $g-3\mu k^2$                                     | Yes        | No          |
| (b)      | $-c^2k^2-\mu k^4+\omega^2=0$     | $\pm\sqrt{c^2+\mu k^2}$            | $\pm\frac{2c^2k+4k^3\mu}{2\sqrt{c^2k^2+k^4\mu}}$ | Yes        | Yes         |
| (c)      | $k^2\hbar^2+2m(V-\omega\hbar)=0$ | $\frac{k^2\hbar^2+2mV}{2m\hbar k}$ | $\frac{k\hbar}{m}$                               | Yes        | No          |

### Question (a)

$$
u_t+gu_x+\mu u_{xxx}=0
$$

With the plane wave solution

$$
u(x,t)=e^{I(kx-\omega t)},
$$

we have

$$
I g k e^{I (k x-t \omega )}-I k^3 \mu  e^{I (k x-t \omega )}-I \omega  e^{I (k x-t \omega )}=0.
$$

That simplifies to

$$
\left(-g k+k^3 \mu +\omega \right) e^{I (k x-t \omega )}=0
$$

which holds for all $x,t$ if and only if

$$
-g k+k^3 \mu +\omega =0,\label{eq1}
$$

and this is the dispersion relation. The phase velocity

$$
v_{ph}=\frac{\re\omega}{k}=g+\mu k^2.
$$

The group velocity

$$
v_{g}=\frac{\d\omega}{\d k}=g-3\mu k^2.
$$

The equation is dispersive since $v_{ph}$ depends on $k$. The equation is nondissipative since $(\ref{eq1})$ requires $\im\omega$ to be zero.

### Question (b)

$$
c^2u_{xx}=u_{tt}+\mu u_{xxxx}
$$

With the plane wave solution, we have

$$
-c^2 k^2 e^{I (k x-t \omega )}=k^4 \mu  e^{I (k x-t \omega )}-\omega ^2 e^{I (k x-t \omega )}.
$$

That simplifies to

$$
\left(-c^2 k^2+k^4 (-\mu )+\omega ^2\right) e^{I (k x-t \omega )}=0.
$$

Therefore the dispersion relation is

$$
-c^2 k^2-\mu k^4+\omega ^2=0\implies w^2=c^2k^2+\mu k^4.\label{eq2}
$$

Since $k,\mu,c$ are all real, $\omega$ is real. The phase velocity

The phase velocity

$$
v_{ph}=\frac{\re\omega}{k}=\pm\sqrt{c^2+\mu k^2}.
$$

The group velocity

$$
v_g=\frac{\d\omega}{\d k}=\pm\frac{2 c^2 k+4 k^3 \mu }{2 \sqrt{c^2 k^2+k^4 \mu }}.
$$

It can be shown that

$$
v_g^2=\frac{\left(c^2+2 k^2 \mu \right)^2}{c^2+k^2 \mu }=\frac{(v_{ph}^2+k^2\mu)^2}{v_{ph}^2}=v_{ph}^2+2k^2\mu+\frac{k^4\mu^2}{v_{ph}^2}>v_{ph}^2.
$$

Also,

$$
\begin{aligned}
    &v_g^2<4v_{ph}^2\\
    \iff&\frac{\left(c^2+2 k^2 \mu \right)^2}{c^2+k^2 \mu }<4 \left(c^2+k^2 \mu \right)\\
    \iff&c^2 \left(c^2+k^2 \mu \right) \left(3 c^2+4 k^2 \mu \right)>0
\end{aligned}
$$

which is true since $\mu$ is positive.

The equation is dispersive since $v_{ph}$ depends on $k$. It is also disspative because in $(\ref{eq2})$, $\omega$ is not necessarily real.

### Question (c)

$$
I\hbar u_t=-\frac{\hbar^2}{2m}u_{xx}+Vu.
$$

With the plane wave solution, we have

$$
\omega  \hbar  e^{i (k x-t \omega )}=\frac{k^2 \hbar ^2 e^{i (k x-t \omega )}}{2 m}+V e^{i (k x-t \omega )}
$$

which simplifies to

$$
\frac{e^{i (k x-t \omega )} \left(k^2 \hbar ^2+2 m (V-\omega  \hbar )\right)}{m}=0.
$$

The dispersion relation is

$$
k^2 \hbar ^2+2 m (V-\omega  \hbar )=0.
$$

The phase velocity

$$
v_{ph}=\frac{\re\omega}{k}=\frac{k^2 \hbar ^2+2 m V}{2 m \hbar k}
$$

The group velocity

$$
v_g=\frac{\d\omega}{\d k}=\frac{k \hbar }{m}
$$

The equation is dispersive since $v_{ph}$ depends on $k$. It is also nondissipative since $\im\omega$ is zero.

## Problem 2

![](https://cdn.duanyll.com/img/20240513093745.png)

### Question (a)

$$
u(x,0)=f(x)\implies u_{i,0}=f_i
$$

$$
\begin{aligned}
    u_t(x,0)=g(x)&\implies-\frac{3}{2}u_{i,0}+2u_{i,1}-\frac{1}{2}u_{i,2}=kg_i\\
    &\implies u_{i,2}=4u_{i,1}-3f_i-2kg_i
\end{aligned}\label{eq3}
$$

### Question (b)

From (5.31) we have

$$
u_{i,2}=\lambda^2 u_{i+1,1}+2(1-\lambda^2)u_{i,1}+\lambda^2 u_{i-1,1}-u_{i,0}.\label{eq4}
$$

With the initial condition in $(\ref{eq3})$ we have

$$
4u_{i,1}-3f_i-2kg_i=\lambda^2 u_{i+1,1}+2(1-\lambda^2)u_{i,1}+\lambda^2 u_{i-1,1}-u_{i,0}.
$$

That is 

$$
-\lambda^2 u_{i+1,1}+2(1+\lambda^2)u_{i,1}-\lambda^2 u_{i-1,1}=2(f_i+kg_i).
$$

All desired $u_{i,1}$ can be solved by the tridiagonal matrix equation

$$
\begin{bmatrix}
    2(1+\lambda^2) & -\lambda^2 & 0 & \cdots & 0\\
    -\lambda^2 & 2(1+\lambda^2) & -\lambda^2 & \cdots & 0\\
    0 & -\lambda^2 & 2(1+\lambda^2) & \cdots & 0\\
    \vdots & \vdots & \vdots & \ddots & \vdots\\
    0 & 0 & 0 & \cdots & 2(1+\lambda^2)
\end{bmatrix}\mathbf{u}_1=\begin{bmatrix}
    2(f_1+kg_1)\\
    2(f_2+kg_2)\\
    2(f_3+kg_3)\\
    \vdots\\
    2(f_N+kg_N)
\end{bmatrix}.\label{eq5}
$$

And then compute $u_{i,2}$ using $(\ref{eq4})$, and so on.

### Question (c)

The method satisfies CFL condition, since the system described by $(\ref{eq5})$ requires $u_{i,1}$ depends on all of $u_{i,0}$, so the numerical domain of dependence is the entire domain. As shown in previous chapters, an unnecessarily large domain of dependence can lead to less accurate results. Using other approximations in space can not lift the need to solve the tridiagonal matrix equation.

### Question (d)

$$
u(x,0)=f(x)\implies u_{i,0}=f_i
$$

$$
\begin{aligned}
    u_t(x,0)=g(x)&\implies-\frac{1}{2}u_{i,-1}+\frac{1}{2}u_{i,1}=kg_i\\
    &\implies u_{i,-1}=u_{i,1}-2kg_i
\end{aligned}\label{eq6}
$$

From (5.31) we have

$$
u_{i,1}=\lambda^2u_{i+1,0}+2(1-\lambda^2)u_{i,0}+\lambda^2 u_{i-1,0}-u_{i,-1}.
$$

With the initial condition in $(\ref{eq6})$ we have

$$
u_{i,1}=\lambda^2u_{i+1,0}+2(1-\lambda^2)u_{i,0}+\lambda^2 u_{i-1,0}-u_{i,1}+2kg_i.
$$

Therefore $u_{i,1}$ can be determined explicitly by

$$
u_{i,1}=\frac{1}{2}u_{i+1,0}+(1-\lambda^2)u_{i,0}+\frac{1}{2}u_{i-1,0}+kg_i.
$$

The stencil for $u_{i,1}$ is $u_{i-1,0},u_{i,0},u_{i+1,0}$, which is a 3-point stencil. 

```tikz
\begin{document}
\begin{tikzpicture}
\draw[gray, thick] (-2,0) -- (2,0);
\draw[gray, thick] (-2,-1) -- (2,-1);
\draw[gray, thick] (-1,-1.5) -- (-1,0.5);
\draw[gray, thick] (0,-1.5) -- (0,0.5);
\draw[gray, thick] (1,-1.5) -- (1,0.5);
\draw (-2.5,0) node {$t_{1}$};
\draw (-2.5,-1) node {$t_{0}$};
\draw (-1,-2) node {$x_{i-1}$};
\draw (0,-2) node {$x_i$};
\draw (1,-2) node {$x_{i+1}$};
\draw[red] (0,0) circle [radius=0.15];
\filldraw[red] (-1,-1) circle [radius=0.15];
\filldraw[red] (0,-1) circle [radius=0.15];
\filldraw[red] (1,-1) circle [radius=0.15];
\end{tikzpicture}
\end{document}
```

The CFL condition is the same as in the textbook.

$$
\frac{ck}{h}<1
$$

## Problem 3

![](https://cdn.duanyll.com/img/20240513093812.png)

### Question (a)

1. Use a uniform grid
   $$
   \begin{aligned}
    x_i&=ih,\quad i=0,1,\cdots,N,N+1,\\
    t_j&=jk,\quad j=0,1,\cdots,M,
   \end{aligned}
   $$
   where $k=T/M$ and $h=l/(N+1)$
2. Evaluate the difference equation at $(x_i,t_j)$
   $$
   u_{tt}(x_i,t_j)+u_t(x_i,t_j)=u_{xx}(x_i,t_j).
   $$
3. Using centered differences to approximate the derivatives we have
   $$
   \begin{aligned}
    &\frac{1}{k^2}\big(u(x_{i},t_{j-1})-2u(x_i,t_j)+u(x_i,t_{j+1})\big)\\
    +\;&\frac{1}{k}\left(-\frac{1}{2}u(x_i,t_{j-1})+\frac{1}{2}u(x_i,t_{j+1})\right)+O(k^2)\\
    =\;&\frac{1}{h^2}\big(u(x_{i+1},t_{j})-2u(x_i,t_j)+u(x_{i-1,}t_j)\big)+O(h^2).
   \end{aligned}
   $$
   This can be rearranged to
   $$
   \begin{aligned}
    u(x_i,t_{j+1})&=\frac{k-2}{k+2}u(x_i,t_{j-1})+\frac{2k^2}{(k+2)h^2}u(x_{i-1},t_j)+\frac{4h^2-4k^2}{(k+2)h^2}u(x_i,t_j)\\
    &+\frac{2k^2}{(k+2)h^2}u(x_{i+1},t_j)+k^2\tau_{ij},
   \end{aligned}
   $$
   where $\tau_{ij}=O(k^2+h^2)$ is the truncation error.
4. Drop the error term to get the finite difference approximation
   $$
   u_{i,j+1}=\frac{k-2}{k+2}u_{i,j-1}+\frac{2k^2}{(k+2)h^2}u_{i-1,j}+\frac{4h^2-4k^2}{(k+2)h^2}u_{i,j}+\frac{2k^2}{(k+2)h^2}u_{i+1,j},\label{eq7}
   $$
   for $i=1,2,\cdots,N$ and $j=1,2,\cdots,M-1$. The first boundary condition in (5.2) can be approximated by
   $$
    u_{0,j}=0,\quad u_{N+1,j}=0.
   $$
   The second boundary condition in (5.3) can be handled by introducing ghost points at $t_{-1}$, described in $(\ref{eq6})$. With $(\ref{eq6})$ we can calculate $u_{i,1}$ for $i=1,2,\cdots,N$
   $$
    u_{i,1}=(1-\frac{1}{2}k)g_i+\frac{k^2}{2h^2}f_{i-1}+(h^2-k^2)f_i+\frac{k^2}{2h^2}f_{i+1}.
   $$

The stencil for this method is 

```tikz
\begin{document}
\begin{tikzpicture}
\draw[gray, thick] (-2,1) -- (2,1);
\draw[gray, thick] (-2,0) -- (2,0);
\draw[gray, thick] (-2,-1) -- (2,-1);
\draw[gray, thick] (-1,-1.5) -- (-1,1.5);
\draw[gray, thick] (0,-1.5) -- (0,1.5);
\draw[gray, thick] (1,-1.5) -- (1,1.5);
\draw (-2.5,1) node {$t_{j+1}$};
\draw (-2.5,0) node {$t_j$};
\draw (-2.5,-1) node {$t_{j-1}$};
\draw (-1,-2) node {$x_{i-1}$};
\draw (0,-2) node {$x_i$};
\draw (1,-2) node {$x_{i+1}$};
\draw[red] (0,1) circle [radius=0.15];
\filldraw[red] (1,0) circle [radius=0.15];
\filldraw[red] (0,-1) circle [radius=0.15];
\filldraw[red] (0,0) circle [radius=0.15];
\filldraw[red] (-1,0) circle [radius=0.15];
\end{tikzpicture}
\end{document}
```

and 

```tikz
\begin{document}
\begin{tikzpicture}
\draw[gray, thick] (-2,0) -- (2,0);
\draw[gray, thick] (-2,-1) -- (2,-1);
\draw[gray, thick] (-1,-1.5) -- (-1,0.5);
\draw[gray, thick] (0,-1.5) -- (0,0.5);
\draw[gray, thick] (1,-1.5) -- (1,0.5);
\draw (-2.5,0) node {$t_{1}$};
\draw (-2.5,-1) node {$t_{0}$};
\draw (-1,-2) node {$x_{i-1}$};
\draw (0,-2) node {$x_i$};
\draw (1,-2) node {$x_{i+1}$};
\draw[red] (0,0) circle [radius=0.15];
\filldraw[red] (-1,-1) circle [radius=0.15];
\filldraw[red] (0,-1) circle [radius=0.15];
\filldraw[red] (1,-1) circle [radius=0.15];
\end{tikzpicture}
\end{document}
```

at the first time step The numerical domain of dependence consists of the points

$$
\{x_i-jh,x_i-(j-1)h,\cdots,x_i+(j-1)h,x_i+jh\}.
$$

The domain of dependence of the damped wave equation is

$$
x_i-t_j\leq x\leq x_i+t_j.
$$

To satify the CFL condition, we need

$$
\frac{k}{h}\leq 1.
$$

### Question (b)

Assuming

$$
u_{i,j}=w_je^{rx_iI},
$$

we can substitute this into $(\ref{eq7})$ to obtain

$$
h^2(k-2)w_{j-1}+4(h^2-2k^2\sin^2\frac{hr}{2})w_j-h^2(k+2)w_{j+1}=0.
$$

The amplification factor is

$$
\kappa=\frac{4 h^2\pm\sqrt{4 h^4 k^2-64 h^2 k^2 \sin ^2\left(\frac{h r}{2}\right)+64 k^4 \sin ^4\left(\frac{h r}{2}\right)}-8
   k^2 \sin ^2\left(\frac{h r}{2}\right)}{2 \left(h^2 k+2 h^2\right)}
$$

*From some numerical experiments* we can find that the magnitude of the amplification factor is less than 1 for all positive $k,h,r$. The method is always stable.

### Question (c)

First we investigate the dispersion relation of the damped wave equation

$$
u_{tt}+u_t=u_{xx}.
$$

Substituting the plane wave solution, we have 

$$
\omega ^2 \left(-e^{I (\bar{k} x-t \omega )}\right)+(-I) \omega  e^{I (\bar{k} x-t \omega )}=\bar{k}^2 \left(-e^{I (\bar{k} x-t \omega )}\right),
$$

and the dispersion relation is

$$
\bar{k}^2-\omega(I+\omega)=0.
$$

The phase velocity is

$$
v_{ph}=\frac{\re\omega}{\bar{k}}=\pm\frac{\sqrt{4\bar{k}^2-1}}{2\bar{k}},
$$

and depends on $\bar{k}$. Therefore the damped wave equation is dispersive. $\im \omega$ is not zero, so the equation is dissipative.

Then we investigate the dispersion relation of the finite difference method. The numerical plane wave solution is

$$
u_{i,j}=e^{I(\bar{k}x_i-\bar{\omega} t_j)}
$$

Substituting this into $(\ref{eq7})$ we have

$$
-I h^2 k \sin (k \omega )+2 h^2 \cos (k \omega )-2 h^2-2 k^2 \cos (h \bar{k})+2 k^2=0
$$

It will be difficult to solve $\omega$, but it can be shown that $v_{nph}$ always depends on $\bar{k}$ and $\omega$ has a non-zero imaginary part. Therefore the finite difference method is dispersive and dissipative, matching the properties of the damped wave equation.

## Problem 4

![](https://cdn.duanyll.com/img/20240513094001.png)

![](https://cdn.duanyll.com/img/20240513094250.png)

### Question (a)

$$
E(t)=\frac{1}{2}\int_{0}^{l}(u_t^2+u_x^2)\d x.
$$

$$
\begin{aligned}
    \frac{\p E(t)}{\p t}&=\int_{0}^{l}\frac{\p u}{\p t}\cdot\frac{\p^2 u}{\p t^2}\d x +\int_0^l\frac{\p u}{\p x}\cdot\frac{\p^2 u}{\p x\p t}\d x\\
    &=\int_{0}^{l}\frac{\p u}{\p t}\cdot\frac{\p^2 u}{\p t^2}\d x+\int_0^l\frac{\p u}{\p x}\d\frac{\p u}{\p t}\\
    &=\int_{0}^{l}\frac{\p u}{\p t}\cdot\frac{\p^2 u}{\p t^2}\d x+\left(\frac{\p u}{\p x}\cdot\frac{\p u}{\p t}\right)\bigg|^l_{x=0}-\int_0^l\frac{\p u}{\p t}\d\frac{\p u}{\p x}\\
    &=\int_{0}^{l}\frac{\p u}{\p t}\cdot\frac{\p^2 u}{\p t^2}\d x-\int_0^l\frac{\p u}{\p t}\cdot\frac{\p^2 u}{\p x^2}\d x
\end{aligned}
$$

With the wave equation

$$
\frac{\p^2 u}{\p t^2}=\frac{\p^2 u}{\p x^2},
$$

we have $E'(t)=0$. Therefore $E(t)$ is a constant.

### Question (b)

The discrete energy is

$$
E_h(t)=\frac{u_1^2+u_N^2}{4h}+\frac{h}{2}\sum_{i=1}^n\left((u_i')^2+\frac{(u_{i+1}-u_i)^2+(u_i-u_{i-1})^2}{2h^2}\right),
$$

and the approximation of the wave equation is

$$
u_i''=\frac{1}{h^2}(u_{i+1}-2u_i+u_{i-1}).
$$

$$
\begin{aligned}
    E_h'(t)&=\frac{u_1u_1'+u_2u_2'}{2h}+\frac{h}{2}\sum_{i=1}^n\left(2u_i'u_i''+\frac{(u_{i+1}-u_i)(u_{i+1}'-u_i')+(u_i-u_{i-1})(u_i'-u_{i-1}')}{h^2}\right)\\
    &=\frac{u_1u_1'+u_2u_2'}{2h}+\frac{h}{2}\sum_{i=1}^n\left(\frac{2u_i'(u_{i+1}-2u_i+u_{i-1})}{h^2}+\frac{(u_{i+1}-u_i)u_{i+1}'-(u_{i+1}-2u_i+u_{i-1})u_i'+(u_{i-1}-u_{i})u'_{i-1}}{h^2}\right)\\
    &=\frac{1}{2h}\left(u_1u_1'+u_Nu_N'+\sum_{i=1}^N(u_{i+1}-2u_i+u_{i-1})u_i'+\sum_{i=1}^N(u_{i+1}-u_i)u_{i+1}'+\sum_{i=1}^N(u_{i-1}-u_{i})u'_{i-1}\right)\\
    &=\frac{1}{2h}\left(u_1u_1'+u_Nu_N'+\sum_{i=1}^N(u_{i+1}-2u_i+u_{i-1})u_i'+\sum_{i=2}^{N+1}(u_{i}-u_{i-1})u_{i}'+\sum_{i=0}^{N-1}(u_{i}-u_{i+1})u'_{i}\right)\\
    &=\frac{1}{2h}\left(u_1u_1'+u_Nu_N'+(u_0-u_1)u_1'+(u_{N+1}-u_N)u_N'\right)\\
    &=\frac{1}{2h}(u_0u_1'+u_{N+1}u_N').
\end{aligned}
$$

From the boundry condition we have $u_0=u_N=0$, so $E_h'(t)=0$. Therefore $E_h(t)$ is a constant.